alloc0

Struct2.v
@@ -6,33 +6,48 @@ Hint Rewrite conseq_cons' : rew_listx.
 
 Open Scope Z_scope.
 
+Section list_of_fun.
+
+Import List.
+
 (* some customized theory of from functions to lists *)
 Lemma list_of_fun [A : Type] [def : A] (f : int -> A) (n : int) (H : 0 <= n) :
   @sigT (list A) (fun l =>
-    (List.length l = n :> int /\ (forall i : int, 0 <= i < n -> List.nth (abs i) l def = f i))).
+    (length l = n :> int /\ (forall i : int, 0 <= i < n -> nth (abs i) l def = f i))).
 Proof.
   remember (abs n) as nn eqn:E.
   revert n H E. induction nn as [ | nn IH ]; intros.
   { assert (n = 0) as -> by math. exists (@nil A). split; auto. intros; math. }
   { assert (nn = abs (n - 1)) as Hq by math. apply IH in Hq; try math.
-    destruct Hq as (la & H1 & H2). exists (List.app la (f (n - 1) :: nil)).
-    rewrite -> List.app_length. split; simpl; try math.
+    destruct Hq as (la & H1 & H2). exists (app la (f (n - 1) :: nil)).
+    rewrite -> app_length. split; simpl; try math.
     intros i Hin. destruct (Z.leb (n - 1) i) eqn:E2.
     { apply Z.leb_le in E2. replace i with (n-1) in * by math. 
-      replace (abs (n-1)) with (List.length la) by math. now rewrite List.nth_middle. }
-    { apply Z.leb_gt in E2. rewrite List.app_nth1. 1: apply H2. all: math. } }
+      replace (abs (n-1)) with (length la) by math. now rewrite nth_middle. }
+    { apply Z.leb_gt in E2. rewrite app_nth1. 1: apply H2. all: math. } }
 Qed.
 
 Definition intlist_of_intfun (f : int -> int) (n : int) :
   @sigT (list int) (fun l =>
-    (List.length l = abs n :> int /\ (forall i : int, 0 <= i < abs n -> List.nth (abs i) l 0 = f i))).
+    (length l = abs n :> int /\ (forall i : int, 0 <= i < abs n -> nth (abs i) l 0 = f i))).
 apply list_of_fun. math. Defined.
+
+Fact lof_make_constfun (n c : int) (H : 0 <= n) :
+  (projT1 (intlist_of_intfun (fun=> c) n)) = repeat c (abs n).
+Proof.
+  destruct (intlist_of_intfun _ _) as (l & Hlen & HH). simpl.
+  apply nth_ext with (d:=0) (d':=0).
+  1: rewrite repeat_length; math.
+  intros i Hi. rewrite -> nth_indep with (l:=repeat _ _) (d':=c) by (rewrite repeat_length; math).
+  rewrite -> nth_repeat, <- HH with (i:=i); try math.
+  f_equal; math.
+Qed.
+
+End list_of_fun.
 
 (* codomain restricted to be int; TODO make n int or nat here? *)
 Definition harray_fun {D : Type} (f:int -> int) (p:loc) (n:int) (d : D) : hhprop D :=
   harray_int (projT1 (intlist_of_intfun f n)) p d.
-
-(* TODO possibly, some conversions between harray_int and harray_fun *)
 
 Section alloc0.
 
@@ -40,9 +55,7 @@ Definition memset0 : val := Eval cbn zeta beta in
   let whilecond (i len : trm) := <{ let 'o = ! i in let 'c = 'o < len in 'c }> in
   let loopbody (p i : trm) := 
     <{ let 'o = ! i in
-       let 'a = val_ptr_add p 1 in 
-       let 'a = val_ptr_add 'a 'o in 
-       'a := 0;
+       val_array_set p 'o 0;
        ++ i }> in
   let loop := While (whilecond "i" "l") (loopbody "p" "i") in
   <{ fun 'p =>
@@ -52,17 +65,78 @@ Definition memset0 : val := Eval cbn zeta beta in
       free 'i }>.
 
 Ltac fold' := 
-  rewrite ?wp_single
+  rewrite ?wp_single ?length_List_length
     -/(incr1.func _) 
     -/(While_aux _ _) 
     -/(While _ _) //=.
-(*
+
+Import List.
+
+Fact list_update_intermediate (L : list val) (i : int) (H : 0 <= i < length L) :
+  (List.app (repeat (val_int 0) (abs (i+1))) (skipn (abs (i+1)) L)) =
+  LibList.update (abs i) (val_int 0) (List.app (repeat (val_int 0) (abs i)) (skipn (abs i) L)).
+Admitted.
+
+(* TODO move this to somewhere else *)
+Fact map_conversion [A B : Type] (l : list A) (f : A -> B) :
+  LibList.map f l = map f l.
+Proof.
+  induction l; simpl; rewrite ?LibList.map_cons ?LibList.map_nil; auto; f_equal; auto.
+Qed.
+
 Lemma htriple_memset0_unary {D : Type} `{Inhab D} (L : list val) (p : loc) (d : D) :
   htriple (single d tt) (fun=> memset0 p)
     (harray L p d) 
-    (fun=> harray_fun (fun=> 0) p (List.length L) d).
+    (fun=> harray_fun (fun=> 0) p (length L) d).
 Proof with fold'.
   xwp; xapp (@htriple_array_length)...
-  xwp; xapp=> s.
-*)
+  xwp; xapp=> s...
+  remember (s d) as s0 eqn:Es0. (* ? *)
+  xwp; xwhile1 0 (length L) (match L with nil => false | _ => true end)
+    (fun (b : bool) (i : int) => \[i <= (length L) /\ Z.ltb i (length L) = b] \*
+      s0 ~(d)~> i \* 
+      harray (List.app (repeat (val_int 0) (abs i)) (skipn (abs i) L)) p d); try math.
+  { intros b i. xsimpl. intros (Hi & Eb).
+    do 2 (xwp; xapp). xwp. xval. xsimpl*. rewrite isTrue_eq_if.
+    case_if; rewrite <- ? Z.ltb_ge, <- ? Z.ltb_lt, -> ? Eb in *; by destruct b. }
+  { intros i. xsimpl*. rewrite Z.ltb_ge. math. }
+  { intros i. xsimpl*. rewrite Z.ltb_lt. math. }
+  { intros i Hii IH. xsimpl*=>_.
+    xwp. xseq. xwp; xapp. 
+    xwp; xapp (@htriple_array_set)...
+    1:{ intros _ _... rewrite app_length repeat_length skipn_length; math. }
+    xapp @incr1.spec.
+    replace (harray _ p d)  (* TODO why simply rewriting does not work? *)
+      with (harray (List.app (repeat (val_int 0) (abs (i+1))) (skipn (abs (i+1)) L)) p d) at 1.
+    2: f_equal; now apply list_update_intermediate. 
+    xapp IH; try math.
+    1: split; [ math | reflexivity ].
+    xsimpl*. }
+  { xsimpl*. split; try math. destruct L; by rewrite ? Z.ltb_ge ? Z.ltb_lt. }
+  { xsimpl*=> _ _. xwp; xapp. 
+    replace (abs _) with (length L) by math. (* ... *)
+    rewrite skipn_all List.app_nil_r /harray_fun /harray_int lof_make_constfun; try math.
+    (* shall we abort LibList.map? *)
+    rewrite map_conversion map_repeat. 
+    replace (abs _) with (length L) by math. (* ... *) xsimpl*. }
+Qed.
+
+Definition alloc0 : val :=
+  <{ fun 'n => 
+      let 'p = val_alloc 'n in
+      memset0 'p; 
+      'p }>.
+
+Lemma htriple_alloc0_unary {D : Type} `{Inhab D} (n : int) (d : D) (Hn : 0 <= n) :
+  htriple (single d tt) (fun=> alloc0 n)
+    \[]
+    (fun hv => \exists p, \[hv d = val_loc p] \* harray_fun (fun=> 0) p n d).
+Proof with fold'.
+  assert (n = abs n :> int) as E by math.
+  rewrite -> E.
+  xwp; xapp (@htriple_alloc_nat)=>x p EE... rewrite !EE.
+  xwp; xapp (@htriple_memset0_unary). xwp; xval. xsimpl*.
+  rewrite -length_List_length length_make. xsimpl.
+Qed.
+
 End alloc0.
